src/FlatImp.v
@@ -13,6 +13,8 @@ Section FlatImp1.
 
   Context {Name: NameWithEq}.
   Notation var := (@name Name).
+  Context {FName : NameWithEq}.
+  Notation func := (@name FName).
   Existing Instance eq_name_dec.
 
   Context {state: Type}.
@@ -31,7 +33,146 @@ Section FlatImp1.
     | SIf(cond: var)(bThen bElse: stmt): stmt
     | SLoop(body1: stmt)(cond: var)(body2: stmt): stmt
     | SSeq(s1 s2: stmt): stmt
-    | SSkip: stmt.
+    | SSkip: stmt
+    | SCall(binds: list var)(f: func)(args: list var).
+
+  Section WithEnv.
+    Context {env} {funcMap: Map env func (list var * list var * stmt)} (e:env).
+
+    (* If we want a bigstep evaluation relation, we either need to put
+       fuel into the SLoop constructor, or give it as argument to eval *)
+    Fixpoint eval_stmt(f: nat)(st: state)(m: mem)(s: stmt): option (state * mem) :=
+      match f with
+      | 0 => None (* out of fuel *)
+      | S f => match s with
+        | SLoad x a =>
+            a <- get st a;
+            v <- read_mem a m;
+            Return (put st x v, m)
+        | SStore a v =>
+            a <- get st a;
+            v <- get st v;
+            m <- write_mem a v m;
+            Return (st, m)
+        | SLit x v =>
+            Return (put st x v, m)
+        | SOp x op y z =>
+            y <- get st y;
+            z <- get st z;
+            Return (put st x (eval_binop op y z), m)
+        | SSet x y =>
+            v <- get st y;
+            Return (put st x v, m)
+        | SIf cond bThen bElse =>
+            vcond <- get st cond;
+            eval_stmt f st m (if dec (vcond = $0) then bElse else bThen)
+        | SLoop body1 cond body2 =>
+            p <- eval_stmt f st m body1;
+            let '(st, m) := p in
+            vcond <- get st cond;
+            if dec (vcond = $0) then Return (st, m) else
+              q <- eval_stmt f st m body2;
+              let '(st, m) := q in
+              eval_stmt f st m (SLoop body1 cond body2)
+        | SSeq s1 s2 =>
+            p <- eval_stmt f st m s1;
+            let '(st, m) := p in
+            eval_stmt f st m s2
+        | SSkip => Return (st, m)
+        | SCall binds fname args =>
+          fimpl <- get e fname;
+          let '(params, rets, fbody) := fimpl in
+          argvs <- option_all (map (get st) args);
+          st0 <- putmany params argvs empty;
+          st1m' <- eval_stmt f st0 m fbody;
+          let '(st1, m') := st1m' in
+          retvs <- option_all (map (get st1) rets);
+          st' <- putmany binds retvs st;
+          Return (st', m')
+        end
+      end.
+
+    Local Ltac inversion_lemma :=
+      intros;
+      simpl in *;
+      repeat (destruct_one_match_hyp; try discriminate);
+      inversionss;
+      eauto 16.
+
+    Lemma invert_eval_SLoad: forall fuel initialSt initialM x y final,
+      eval_stmt (S fuel) initialSt initialM (SLoad x y) = Some final ->
+      exists a v, get initialSt y = Some a /\
+                  read_mem a initialM = Some v /\
+                  final = (put initialSt x v, initialM).
+    Proof. inversion_lemma. Qed.
+
+    Lemma invert_eval_SStore: forall fuel initialSt initialM x y final,
+      eval_stmt (S fuel) initialSt initialM (SStore x y) = Some final ->
+      exists a v finalM, get initialSt x = Some a /\
+                         get initialSt y = Some v /\
+                         write_mem a v initialM = Some finalM /\
+                         final = (initialSt, finalM).
+    Proof. inversion_lemma. Qed.
+
+    Lemma invert_eval_SLit: forall fuel initialSt initialM x v final,
+      eval_stmt (S fuel) initialSt initialM (SLit x v) = Some final ->
+      final = (put initialSt x v, initialM).
+    Proof. inversion_lemma. Qed.
+
+    Lemma invert_eval_SOp: forall fuel x y z op initialSt initialM final,
+      eval_stmt (S fuel) initialSt initialM (SOp x op y z) = Some final ->
+      exists v1 v2,
+        get initialSt y = Some v1 /\
+        get initialSt z = Some v2 /\
+        final = (put initialSt x (eval_binop op v1 v2), initialM).
+    Proof. inversion_lemma. Qed.
+
+    Lemma invert_eval_SSet: forall fuel x y initialSt initialM final,
+      eval_stmt (S fuel) initialSt initialM (SSet x y) = Some final ->
+      exists v,
+        get initialSt y = Some v /\ final = (put initialSt x v, initialM).
+    Proof. inversion_lemma. Qed.
+
+    Lemma invert_eval_SIf: forall fuel cond bThen bElse initialSt initialM final,
+      eval_stmt (S fuel) initialSt initialM (SIf cond bThen bElse) = Some final ->
+      exists vcond,
+        get initialSt cond = Some vcond /\
+        (vcond <> $0 /\ eval_stmt fuel initialSt initialM bThen = Some final \/
+         vcond =  $0 /\ eval_stmt fuel initialSt initialM bElse = Some final).
+    Proof. inversion_lemma. Qed.
+
+    Lemma invert_eval_SLoop: forall fuel st1 m1 body1 cond body2 p4,
+      eval_stmt (S fuel) st1 m1 (SLoop body1 cond body2) = Some p4 ->
+      eval_stmt fuel st1 m1 body1 = Some p4 /\ get (fst p4) cond = Some $0 \/
+      exists st2 m2 st3 m3 cv, eval_stmt fuel st1 m1 body1 = Some (st2, m2) /\
+                               get st2 cond = Some cv /\ cv <> $0 /\
+                               eval_stmt fuel st2 m2 body2 = Some (st3, m3) /\
+                               eval_stmt fuel st3 m3 (SLoop body1 cond body2) = Some p4.
+    Proof. inversion_lemma. Qed.
+
+    Lemma invert_eval_SSeq: forall fuel initialSt initialM s1 s2 final,
+      eval_stmt (S fuel) initialSt initialM (SSeq s1 s2) = Some final ->
+      exists midSt midM, eval_stmt fuel initialSt initialM s1 = Some (midSt, midM) /\
+                         eval_stmt fuel midSt midM s2 = Some final.
+    Proof. inversion_lemma. Qed.
+
+    Lemma invert_eval_SSkip: forall fuel initialSt initialM final,
+      eval_stmt (S fuel) initialSt initialM SSkip = Some final ->
+      final = (initialSt, initialM).
+    Proof. inversion_lemma. Qed.
+
+    Lemma invert_eval_SCall : forall st m1 p2 f binds fname args,
+      eval_stmt (S f) st m1 (SCall binds fname args) = Some p2 ->
+      exists params rets fbody argvs st0 st1 m' retvs st',
+        get e fname = Some (params, rets, fbody) /\
+        option_all (map (get st) args) = Some argvs /\
+        putmany params argvs empty = Some st0 /\
+        eval_stmt f st0 m1 fbody = Some (st1, m') /\
+        option_all (map (get st1) rets) = Some retvs /\
+        putmany binds retvs st = Some st' /\
+        p2 = (st', m').
+    Proof. inversion_lemma. Qed.
+  End WithEnv.
 
   Fixpoint stmt_size(s: stmt): nat :=
     match s with
@@ -44,49 +185,7 @@ Section FlatImp1.
     | SLoop body1 cond body2 => 1 + (stmt_size body1) + (stmt_size body2)
     | SSeq s1 s2 => 1 + (stmt_size s1) + (stmt_size s2)
     | SSkip => 1
-    end.
-
-  (* If we want a bigstep evaluation relation, we either need to put
-     fuel into the SLoop constructor, or give it as argument to eval *)
-  Fixpoint eval_stmt(f: nat)(st: state)(m: mem)(s: stmt): option (state * mem) :=
-    match f with
-    | 0 => None (* out of fuel *)
-    | S f => match s with
-      | SLoad x a =>
-          a <- get st a;
-          v <- read_mem a m;
-          Return (put st x v, m)
-      | SStore a v =>
-          a <- get st a;
-          v <- get st v;
-          m <- write_mem a v m;
-          Return (st, m)
-      | SLit x v =>
-          Return (put st x v, m)
-      | SOp x op y z =>
-          y <- get st y;
-          z <- get st z;
-          Return (put st x (eval_binop op y z), m)
-      | SSet x y =>
-          v <- get st y;
-          Return (put st x v, m)
-      | SIf cond bThen bElse =>
-          vcond <- get st cond;
-          eval_stmt f st m (if dec (vcond = $0) then bElse else bThen)
-      | SLoop body1 cond body2 =>
-          p <- eval_stmt f st m body1;
-          let '(st, m) := p in
-          vcond <- get st cond;
-          if dec (vcond = $0) then Return (st, m) else
-            q <- eval_stmt f st m body2;
-            let '(st, m) := q in
-            eval_stmt f st m (SLoop body1 cond body2)
-      | SSeq s1 s2 =>
-          p <- eval_stmt f st m s1;
-          let '(st, m) := p in
-          eval_stmt f st m s2
-      | SSkip => Return (st, m)
-      end
+    | SCall binds f args => S (length binds + length args)
     end.
 
   (* returns the set of modified vars *)
@@ -104,6 +203,7 @@ Section FlatImp1.
     | SSeq s1 s2 =>
         union (modVars s1) (modVars s2)
     | SSkip => empty_set
+    | SCall binds func args => of_list binds
     end.
 
   Fixpoint accessedVars(s: stmt): vars :=
@@ -120,6 +220,7 @@ Section FlatImp1.
     | SSeq s1 s2 =>
         union (accessedVars s1) (accessedVars s2)
     | SSkip => empty_set
+    | SCall binds func args => union (of_list binds) (of_list args)
     end.
 
   Lemma modVars_subset_accessedVars: forall s,
@@ -127,82 +228,12 @@ Section FlatImp1.
   Proof.
     intro s. induction s; simpl; unfold singleton_set; state_calc.
   Qed.
-
-  Local Ltac inversion_lemma :=
-    intros;
-    simpl in *;
-    repeat (destruct_one_match_hyp; try discriminate);
-    inversionss;
-    eauto 15.
-
-  Lemma invert_eval_SLoad: forall fuel initialSt initialM x y final,
-    eval_stmt (S fuel) initialSt initialM (SLoad x y) = Some final ->
-    exists a v, get initialSt y = Some a /\
-                read_mem a initialM = Some v /\
-                final = (put initialSt x v, initialM).
-  Proof. inversion_lemma. Qed.
-
-  Lemma invert_eval_SStore: forall fuel initialSt initialM x y final,
-    eval_stmt (S fuel) initialSt initialM (SStore x y) = Some final ->
-    exists a v finalM, get initialSt x = Some a /\
-                       get initialSt y = Some v /\
-                       write_mem a v initialM = Some finalM /\
-                       final = (initialSt, finalM).
-  Proof. inversion_lemma. Qed.
-
-  Lemma invert_eval_SLit: forall fuel initialSt initialM x v final,
-    eval_stmt (S fuel) initialSt initialM (SLit x v) = Some final ->
-    final = (put initialSt x v, initialM).
-  Proof. inversion_lemma. Qed.
-
-  Lemma invert_eval_SOp: forall fuel x y z op initialSt initialM final,
-    eval_stmt (S fuel) initialSt initialM (SOp x op y z) = Some final ->
-    exists v1 v2,
-      get initialSt y = Some v1 /\
-      get initialSt z = Some v2 /\
-      final = (put initialSt x (eval_binop op v1 v2), initialM).
-  Proof. inversion_lemma. Qed.
-
-  Lemma invert_eval_SSet: forall fuel x y initialSt initialM final,
-    eval_stmt (S fuel) initialSt initialM (SSet x y) = Some final ->
-    exists v,
-      get initialSt y = Some v /\ final = (put initialSt x v, initialM).
-  Proof. inversion_lemma. Qed.
-
-  Lemma invert_eval_SIf: forall fuel cond bThen bElse initialSt initialM final,
-    eval_stmt (S fuel) initialSt initialM (SIf cond bThen bElse) = Some final ->
-    exists vcond,
-      get initialSt cond = Some vcond /\
-      (vcond <> $0 /\ eval_stmt fuel initialSt initialM bThen = Some final \/
-       vcond =  $0 /\ eval_stmt fuel initialSt initialM bElse = Some final).
-  Proof. inversion_lemma. Qed.
-
-  Lemma invert_eval_SLoop: forall fuel st1 m1 body1 cond body2 p4,
-    eval_stmt (S fuel) st1 m1 (SLoop body1 cond body2) = Some p4 ->
-    eval_stmt fuel st1 m1 body1 = Some p4 /\ get (fst p4) cond = Some $0 \/
-    exists st2 m2 st3 m3 cv, eval_stmt fuel st1 m1 body1 = Some (st2, m2) /\
-                             get st2 cond = Some cv /\ cv <> $0 /\
-                             eval_stmt fuel st2 m2 body2 = Some (st3, m3) /\
-                             eval_stmt fuel st3 m3 (SLoop body1 cond body2) = Some p4.
-  Proof. inversion_lemma. Qed.
-
-  Lemma invert_eval_SSeq: forall fuel initialSt initialM s1 s2 final,
-    eval_stmt (S fuel) initialSt initialM (SSeq s1 s2) = Some final ->
-    exists midSt midM, eval_stmt fuel initialSt initialM s1 = Some (midSt, midM) /\
-                       eval_stmt fuel midSt midM s2 = Some final.
-  Proof. inversion_lemma. Qed.
-
-  Lemma invert_eval_SSkip: forall fuel initialSt initialM final,
-    eval_stmt (S fuel) initialSt initialM SSkip = Some final ->
-    final = (initialSt, initialM).
-  Proof. inversion_lemma. Qed.
-
 End FlatImp1.
 
 
 Ltac invert_eval_stmt :=
   lazymatch goal with
-  | E: eval_stmt (S ?fuel) _ _ ?s = Some _ |- _ =>
+  | E: eval_stmt _ (S ?fuel) _ _ ?s = Some _ |- _ =>
     destruct s;
     [ apply invert_eval_SLoad in E
     | apply invert_eval_SStore in E
@@ -212,7 +243,8 @@ Ltac invert_eval_stmt :=
     | apply invert_eval_SIf in E
     | apply invert_eval_SLoop in E
     | apply invert_eval_SSeq in E
-    | apply invert_eval_SSkip in E ];
+    | apply invert_eval_SSkip in E
+    | apply invert_eval_SCall in E ];
     deep_destruct E;
     [ let x := fresh "Case_SLoad" in pose proof tt as x; move x at top
     | let x := fresh "Case_SStore" in pose proof tt as x; move x at top
@@ -224,7 +256,8 @@ Ltac invert_eval_stmt :=
     | let x := fresh "Case_SLoop_Done" in pose proof tt as x; move x at top
     | let x := fresh "Case_SLoop_NotDone" in pose proof tt as x; move x at top
     | let x := fresh "Case_SSeq" in pose proof tt as x; move x at top
-    | let x := fresh "Case_SSkip" in pose proof tt as x; move x at top ]
+    | let x := fresh "Case_SSkip" in pose proof tt as x; move x at top
+    | let x := fresh "Case_SCall" in pose proof tt as x; move x at top ]
   end.
 
 
@@ -235,25 +268,29 @@ Section FlatImp2.
   Context {Name: NameWithEq}.
   Notation var := (@name Name).
   Existing Instance eq_name_dec.
+  Context {FName : NameWithEq}.
+  Notation func := (@name FName).
 
   Context {state: Type}.
   Context {stateMap: Map state var (word wXLEN)}.
   Context {vars: Type}.
   Context {varset: set vars var}.
 
+  Context {env} {funcMap: Map env func (list var * list var * stmt)}.
+
   Ltac state_calc := state_calc_generic (@name Name) (word wXLEN).
 
-  Lemma increase_fuel_still_Success: forall fuel1 fuel2 initialSt initialM s final,
+  Lemma increase_fuel_still_Success: forall fuel1 fuel2 e initialSt initialM s final,
     fuel1 <= fuel2 ->
-    eval_stmt fuel1 initialSt initialM s = Some final ->
-    eval_stmt fuel2 initialSt initialM s = Some final.
+    eval_stmt e fuel1 initialSt initialM s = Some final ->
+    eval_stmt e fuel2 initialSt initialM s = Some final.
   Proof.
     induction fuel1; introv L Ev.
     - inversions Ev.
     - destruct fuel2; [omega|].
       assert (fuel1 <= fuel2) as F by omega. specialize IHfuel1 with (1 := F).
       destruct final as [finalSt finalM].
-      invert_eval_stmt; simpl in *;
+      invert_eval_stmt; cbn in *;
       repeat match goal with
       | IH: _, H: _ |- _ =>
           let IH' := fresh IH in pose proof IH as IH';
@@ -268,8 +305,8 @@ Section FlatImp2.
       eauto.
   Qed.
 
-  Lemma modVarsSound: forall fuel s initialSt initialM finalSt finalM,
-    eval_stmt fuel initialSt initialM s = Some (finalSt, finalM) ->
+  Lemma modVarsSound: forall fuel e s initialSt initialM finalSt finalM,
+    eval_stmt e fuel initialSt initialM s = Some (finalSt, finalM) ->
     only_differ initialSt (modVars s) finalSt.
   Proof.
     induction fuel; introv Ev.
@@ -283,9 +320,8 @@ Section FlatImp2.
           ensure_new IH'
       end;
       state_calc.
+      refine (only_differ_putmany _ _ _ _ _ _); eassumption.
   Qed.
-
-
 End FlatImp2.
 
 Require riscv.RiscvBitWidths32.
@@ -330,7 +366,7 @@ Example fib(n: word 32) :=
               (SOp _n OMinus _n _one)))))
   )))).
 
-Definition eval_stmt_test fuel initialSt := @eval_stmt _ ZName _ _ fuel initialSt no_mem.
+Definition eval_stmt_test fuel initialSt := @eval_stmt _ ZName ZName _ _ _ _ empty fuel initialSt no_mem.
 
 Example finalFibState(n: nat) := (eval_stmt_test 100 empty (fib $n)).
 Example finalFibVal(n: nat): option (word 32) := match finalFibState n with
